par_pass_simu.v

omp_compiler/par_pass_simu.v
@@ -1,5 +1,6 @@
+(* par_pass_simu.v *)
 
-(*
+(***
 From omp_compiler Require Import common par_pass simulation.
 
 Section ParPassSimulation.
@@ -15,60 +16,418 @@ Section ParPassSimulation.
 End ParPassSimulation.
 
 
-*)
+***)
+
+
 
 From omp_compiler Require Import
   common
   par_pass
   simulation.
 
+
+From compcert Require Import
+  Values
+  Clight
+  Ctypes
+  Globalenvs.
+
 From VST.concurrency.openmp_sem Require Import
   DryHybridMachineInst
-  finThreadPool.
+  finThreadPool
+  HybridMachine
+  HybridMachineSig
+  team_dyn.
 
-From compcert.cfrontend Require Import Clight.
+From compcert Require Import
+  Values
+  Clight
+  Memory
+  Ctypes
+  Globalenvs
+  Integers.
 
+Import HybridMachineSig.
 Import finThreadPool.ThreadPool.
+Import FinPool.
 
 Section ParPassSimulation.
 
-  Context
-    (par_state_match :
-       forall {sp tp : program},
-         @Ostate (Clight.globalenv sp) _ ->
-         @Ostate (Clight.globalenv tp) _ ->
-         Prop).
+  (* ================================================================ *)
+  (* Programs and machine states                                      *)
+  (* ================================================================ *)
+
+  Definition SrcState (sp : Clight.program) : Type :=
+    @Ostate (Clight.globalenv sp) _.
+
+  Definition TgtState (tp : Clight.program) : Type :=
+    @Ostate (Clight.globalenv tp) _.
+
+  Definition par_initial_state
+    (p : Clight.program)
+    (st : @Ostate (Clight.globalenv p) _) : Prop :=
+    @init_Ostate (Build_Prog p) st.
+
+  Definition state_schedule
+    {p : Clight.program}
+    (st : @Ostate (Clight.globalenv p) _) :=
+    let '((U, _, _, _), _) := st in U.
+
+  Definition state_trace
+    {p : Clight.program}
+    (st : @Ostate (Clight.globalenv p) _) :=
+    let '((_, tr, _, _), _) := st in tr.
+
+  Definition state_thread_pool
+    {p : Clight.program}
+    (st : @Ostate (Clight.globalenv p) _) :=
+    let '((_, _, tp, _), _) := st in tp.
+
+  Definition state_team_tree
+    {p : Clight.program}
+    (st : @Ostate (Clight.globalenv p) _) :=
+    let '((_, _, _, tree), _) := st in tree.
+
+  (* ================================================================ *)
+  (*  OMP parallel region              *)
+  (* ================================================================ *)
+
+  Inductive par_phase : Type :=
+  | ParSource
+  | ParSetup
+  | ParSpawning
+  | ParParallel
+  | ParJoining
+  | ParFinished.
+
+  (* ================================================================ *)
+  (* Concrete compiler relations                                      *)
+  (* ================================================================ *)
+
+  Definition translated_function
+    (sf tf : function) : Prop :=
+    exists
+      (ids ids' : list ident)
+      (generated_functions :
+         list
+           (ident *
+            globdef (Ctypes.fundef function) Ctypes.type))
+      (generated_composites : list composite_definition),
+      omp_compiler.par_pass.transl_globdef
+        (Gfun (Ctypes.Internal sf))
+        ids
+      =
+        (Gfun (Ctypes.Internal tf),
+         ids',
+         generated_functions,
+         generated_composites).
+
+  Definition translated_statement
+    (temps : list (ident * Ctypes.type))
+    (ss ts : statement) : Prop :=
+    exists
+      (ids ids' : list ident)
+      (generated_functions :
+         list
+           (ident *
+            globdef (Ctypes.fundef function) Ctypes.type))
+      (generated_composites : list composite_definition),
+      omp_compiler.par_pass.transl_Spragma
+        temps ss ids [] []
+      =
+        (ts, ids', generated_functions, generated_composites).
+
+  Definition translated_parallel_statement
+    (nt : nat)
+    (pc pc_first : privatization_clause_type)
+    (rcs : list reduction_clause_type)
+    (pi : pragma_info)
+    (body target_body : statement)
+    (temps : list (ident * Ctypes.type)) : Prop :=
+    exists
+      (ids ids' : list ident)
+      (generated_function :
+         ident * globdef (Ctypes.fundef function) Ctypes.type)
+      (generated_composite : composite_definition),
+      omp_compiler.par_pass.par_pass_s
+        nt pc pc_first rcs pi body ids temps
+      =
+        (target_body,
+         ids',
+         generated_function,
+         generated_composite).
+
+Check Ctypes.External.
+Check @Ctypes.External.
+
+Inductive clight_state_match
+  (sp tp : Clight.program)
+  (Htrans :
+     omp_compiler.par_pass.transl_program sp = Some tp)
+  : Clight_core.state ->
+    Clight_core.state ->
+    Prop :=
+
+| clight_match_state :
+    forall
+      (sf tf : function)
+      (ss ts : statement)
+      (k : cont)
+      (e : env)
+      (le : temp_env),
+
+      translated_function sf tf ->
+
+      translated_statement
+        sf.(fn_temps)
+        ss
+        ts ->
+
+      clight_state_match sp tp Htrans
+        (Clight_core.State
+           sf
+           ss
+           k
+           e
+           le)
+
+        (Clight_core.State
+           tf
+           ts
+           k
+           e
+           le)
+
+| clight_match_callstate_internal :
+    forall
+      (sf tf : function)
+      (args : list val)
+      (k : cont),
+
+      translated_function sf tf ->
+
+      clight_state_match sp tp Htrans
+        (Clight_core.Callstate
+           (@Ctypes.Internal function sf)
+           args
+           k)
+
+        (Clight_core.Callstate
+           (@Ctypes.Internal function tf)
+           args
+           k)
+
+| clight_match_callstate_external :
+    forall
+      (ef : external_function)
+      (targs : typelist)
+      (tres : type)
+      (cc : calling_convention)
+      (args : list val)
+      (k : cont),
+
+      clight_state_match sp tp Htrans
+        (Clight_core.Callstate
+           (@Ctypes.External
+              function
+              ef
+              targs
+              tres
+              cc)
+           args
+           k)
+
+        (Clight_core.Callstate
+           (@Ctypes.External
+              function
+              ef
+              targs
+              tres
+              cc)
+           args
+           k)
+
+| clight_match_returnstate :
+    forall
+      (v : val)
+      (k : cont),
+
+      clight_state_match sp tp Htrans
+        (Clight_core.Returnstate
+           v
+           k)
+
+        (Clight_core.Returnstate
+           v
+           k)
+
+| clight_match_parallel_pragma :
+    forall
+      (pragma_id nt : nat)
+      (pc pc_first : privatization_clause_type)
+      (rcs : list reduction_clause_type)
+      (pi : pragma_info)
+      (sf tf : function)
+      (body target_body : statement)
+      (k : cont)
+      (e : env)
+      (le : temp_env),
+
+      translated_function sf tf ->
+
+      translated_parallel_statement
+        nt
+        pc
+        pc_first
+        rcs
+        pi
+        body
+        target_body
+        sf.(fn_temps) ->
+
+      clight_state_match sp tp Htrans
+        (Clight_core.Pragmastate
+           pragma_id
+           (OMPParallel
+              nt
+              pc
+              pc_first
+              rcs
+              pi)
+           (sf, body, k, e, le))
+
+        (Clight_core.State
+           tf
+           target_body
+           k
+           e
+           le).
+
+
+  Inductive control_match
+    (sp tp : Clight.program)
+    (Htrans : omp_compiler.par_pass.transl_program sp = Some tp)
+    : @ctl Clight_core.state -> @ctl Clight_core.state -> Prop :=
+
+  | control_match_run :
+      forall sc tc,
+        clight_state_match sp tp Htrans sc tc ->
+        control_match sp tp Htrans (Krun sc) (Krun tc)
+
+  | control_match_blocked :
+      forall sc tc,
+        clight_state_match sp tp Htrans sc tc ->
+        control_match sp tp Htrans (Kblocked sc) (Kblocked tc)
+
+  | control_match_resume :
+      forall sc tc v,
+        clight_state_match sp tp Htrans sc tc ->
+        control_match sp tp Htrans (Kresume sc v) (Kresume tc v)
+
+  | control_match_init :
+      forall vf arg,
+        control_match sp tp Htrans (Kinit vf arg) (Kinit vf arg).
+
+  Definition concrete_thread_pair_match
+    {sp tp : Clight.program}
+    (Htrans : omp_compiler.par_pass.transl_program sp = Some tp)
+    (s : SrcState sp)
+    (t : TgtState tp)
+    (sid tid : nat) : Prop :=
+    exists
+      (Hs : containsThread (state_thread_pool s) sid)
+      (Ht : containsThread (state_thread_pool t) tid),
+      control_match sp tp Htrans
+        (getThreadC Hs)
+        (getThreadC Ht).
+
+  Definition concrete_thread_controls_match
+    {sp tp : Clight.program}
+    (Htrans : omp_compiler.par_pass.transl_program sp = Some tp)
+    (s : SrcState sp)
+    (t : TgtState tp) : Prop :=
+    forall tid,
+      containsThread (state_thread_pool t) tid ->
+      exists sid,
+        concrete_thread_pair_match Htrans s t sid tid.
+
+  Definition concrete_threads_match
+    {sp tp : Clight.program}
+    (phase : par_phase)
+    (s : SrcState sp)
+    (t : TgtState tp) : Prop :=
+    match phase with
+    | ParSource
+    | ParSetup
+    | ParParallel
+    | ParFinished =>
+        FinPool.num_threads (state_thread_pool s) =
+        FinPool.num_threads (state_thread_pool t)
+    | ParSpawning
+    | ParJoining =>
+        (FinPool.num_threads (state_thread_pool s) <=
+         FinPool.num_threads (state_thread_pool t))%nat
+    end.
+
+  (* ================================================================ *)
+  (*  global state relation                                *)
+  (* ================================================================ *)
+
+  Record par_state_match
+    {sp tp : Clight.program}
+    (s : SrcState sp)
+    (t : TgtState tp) : Prop :=
+  {
+    par_match_translation :
+      omp_compiler.par_pass.transl_program sp = Some tp;
+
+    par_match_phase : par_phase;
+
+    par_match_memory :
+      exists f : meminj,
+        Mem.inject f (snd s) (snd t);
+
+    par_match_thread_count :
+      concrete_threads_match par_match_phase s t;
+
+    par_match_thread_controls :
+      concrete_thread_controls_match par_match_translation s t
+  }.
 
   Arguments par_state_match {sp tp} _ _.
 
-  Context
-    (par_initial_state :
-       forall p : program,
-         @Ostate (Clight.globalenv p) _ ->
-         Prop).
+  (* ================================================================ *)
+  (* Main compiler-specific preservation theorem                       *)
+  (* ================================================================ *)
 
-  Context
-    (par_state_match_step :
-       forall
-         (sp tp : program)
-         (s : @Ostate (Clight.globalenv sp) _)
-         (t t' : @Ostate (Clight.globalenv tp) _),
+  Lemma par_step_preservation :
+    forall
+      (sp tp : Clight.program)
+      (s : SrcState sp)
+      (t t' : TgtState tp),
 
-         omp_compiler.par_pass.transl_program sp = Some tp ->
+      omp_compiler.par_pass.transl_program sp = Some tp ->
+      par_state_match s t ->
+      Ostep t t' ->
 
-         par_state_match s t ->
+      exists s',
+        @Osteps
+          (Clight.globalenv sp)
+          _
+          s
+          s' /\
+        par_state_match s' t'.
+  Proof.
+    intros sp tp s t t' Htrans Hmatch Hstep.
 
-         Ostep t t' ->
+    unfold Ostep in Hstep.
+    unfold MachStep in Hstep.
 
-         exists
-           (s' : @Ostate (Clight.globalenv sp) _),
+  Admitted.
 
-           Osteps
-             (p := Build_Prog sp)
-             s
-             s' /\
-
-           par_state_match s' t').
+  (* ================================================================ *)
+  (*  one-step and multi-step theorems                           *)
+  (* ================================================================ *)
 
   Lemma par_pass_back_simu_one_step :
     forall sp tp,
@@ -79,24 +438,9 @@ Section ParPassSimulation.
         tp.
   Proof.
     intros sp tp.
-
     unfold back_simu_one_step.
-
-    intros
-      s
-      t
-      t'
-      Htrans
-      Hmatch
-      Htgt_step.
-
-    eapply par_state_match_step.
-
-    - exact Htrans.
-
-    - exact Hmatch.
-
-    - exact Htgt_step.
+    intros s t t' Htrans Hmatch Hstep.
+    eapply par_step_preservation; eauto.
   Qed.
 
   Theorem par_pass_back_simu :
@@ -109,7 +453,6 @@ Section ParPassSimulation.
         tp.
   Proof.
     intros sp tp.
-
     eapply
       (back_simu_one_step_implies_back_simu
          omp_compiler.par_pass.transl_program
@@ -117,7 +460,6 @@ Section ParPassSimulation.
          par_initial_state
          sp
          tp).
-
     apply par_pass_back_simu_one_step.
   Qed.
 
